Update suggest.lean
This commit resolves the changes between this PR and the previous PR for `library_search`/`suggest`.

src/tactic/suggest.lean
@@ -8,6 +8,8 @@ import data.mllist
 import tactic.solve_by_elim
 
 /-!
+# `suggest` and `library_search`
+
 `suggest` and `library_search` are a pair of tactics for applying lemmas from the library to the
 current goal.
 
@@ -58,7 +60,8 @@ def head_symbol_match.to_string : head_symbol_match → string
 /--
 When we are determining if a given declaration is potentially relevant for the current goal,
 we compute `unfold_head_symbol` on the head symbol of the declaration, producing a list of names.
-We consider the declaration potentially relevant if the head symbol of the goal appears in this list.
+We consider the declaration potentially relevant if the head symbol of the goal appears in this
+list.
 -/
 -- This is a hack.
 meta def unfold_head_symbol : name → list name
@@ -78,7 +81,7 @@ meta def match_head_symbol (hs : name) : expr → option head_symbol_match
                        end
 | (expr.app f _)    := match_head_symbol f
 | (expr.const n _)  := if list.mem hs (unfold_head_symbol n) then some ex else none
-| _ := none
+| _ := if hs = `_ then some ex else none
 
 meta structure decl_data :=
 (d : declaration)
@@ -105,11 +108,13 @@ do env ← get_env,
    return $ env.decl_filter_map (process_declaration hs)
 
 /--
-Apply the lemma `e`, then attempt to close all goals using `solve_by_elim { discharger := discharger }`,
-failing if `close_goals = tt` and there are any goals remaining.
+Apply the lemma `e`, then attempt to close all goals using
+`solve_by_elim { ..opt }`, failing if `close_goals = tt`
+and there are any goals remaining.
 -/
 -- Implementation note: as this is used by both `library_search` and `suggest`,
--- we first run `solve_by_elim` separately on a subset of the goals, whether or not `close_goals` is set,
+-- we first run `solve_by_elim` separately on a subset of the goals,
+-- whether or not `close_goals` is set,
 -- and then if `close_goals = tt`, require that `solve_by_elim { all_goals := tt }` succeeds
 -- on the remaining goals.
 meta def apply_and_solve (close_goals : bool) (opt : by_elim_opt := { }) (e : expr) : tactic unit :=
@@ -124,7 +129,8 @@ try (any_goals (independent_goal >> solve_by_elim { ..opt })) >>
 (done <|>
   -- If there were any goals that we did not attempt solving in the first phase
   -- (because they weren't propositional, or contained a metavariable)
-  -- as a second phase we attempt to solve all remaining goals at once (with backtracking across goals).
+  -- as a second phase we attempt to solve all remaining goals at once
+  -- (with backtracking across goals).
   any_goals (success_if_fail independent_goal) >>
   solve_by_elim { ..opt } <|>
   -- and fail unless `close_goals = ff`
@@ -134,7 +140,8 @@ try (any_goals (independent_goal >> solve_by_elim { ..opt })) >>
 Apply the declaration `d` (or the forward and backward implications separately, if it is an `iff`),
 and then attempt to solve the goal using `apply_and_solve`.
 -/
-meta def apply_declaration (close_goals : bool) (opt : by_elim_opt := { }) (d : decl_data) : tactic unit :=
+meta def apply_declaration (close_goals : bool) (opt : by_elim_opt := { }) (d : decl_data) :
+  tactic unit :=
 let tac := apply_and_solve close_goals opt in
 do (e, t) ← decl_mk_const d.d,
    match d.m with
@@ -178,6 +185,28 @@ open suggest
 
 declare_trace suggest         -- Trace a list of all relevant lemmas
 
+-- Call `apply_declaration`, then prepare the tactic script and
+-- count the number of local hypotheses used.
+private meta def apply_declaration_script
+  (g : expr) (hyps : list expr)
+  (opt : by_elim_opt := { })
+  (d : decl_data) :
+  tactic application :=
+-- (This tactic block is only executed when we evaluate the mllist,
+-- so we need to do the `focus1` here.)
+retrieve $ focus1 $ do
+  apply_declaration ff opt d,
+  ng ← num_goals,  
+  s ← read,
+  m ← tactic_statement g,
+  return
+  { application .
+    state := s,
+    decl := d.d,
+    script := m,
+    num_goals := ng,
+    hyps_used := hyps.countp (λ h, h.occurs g) }
+
 -- implementation note: we produce a `tactic (mllist tactic application)` first,
 -- because it's easier to work in the tactic monad, but in a moment we squash this
 -- down to an `mllist tactic application`.
@@ -187,11 +216,11 @@ do g :: _ ← get_goals,
    hyps ← local_context,
 
    -- Make sure that `solve_by_elim` doesn't just solve the goal immediately:
-   (lock_tactic_state (do
+   (retrieve (do
      focus1 $ solve_by_elim { ..opt },
      s ← read,
      m ← tactic_statement g,     
-     return $ mllist.of_list [⟨s, m, none, 0, hyps.countp(λ h, h.occurs g)⟩])) <|>
+     return $ mllist.of_list [⟨s, m, none, 0, hyps.countp (λ h, h.occurs g)⟩])) <|>
    -- Otherwise, let's actually try applying library lemmas.
    (do
    -- Collect all definitions with the correct head symbol
@@ -199,27 +228,25 @@ do g :: _ ← get_goals,
    defs ← library_defs (head_symbol t),
    -- Sort by length; people like short proofs
    let defs := defs.qsort(λ d₁ d₂, d₁.l ≤ d₂.l),
-   when (is_trace_enabled_for `suggest) $ (do
-     trace format!"Found {defs.length} relevant lemmas:",
-     trace $ defs.map (λ ⟨d, n, m, l⟩, (n, m.to_string))),
+   trace_if_enabled `suggest format!"Found {defs.length} relevant lemmas:",
+   trace_if_enabled `suggest $ defs.map (λ ⟨d, n, m, l⟩, (n, m.to_string)),
+
+   let defs : mllist tactic _ := mllist.of_list defs,
 
    -- Try applying each lemma against the goal,
-   -- then record the number of remaining goals, and number of local hypotheses used.
-   return $ (mllist.of_list defs).mfilter_map
-   -- (This tactic block is only executed when we evaluate the mllist,
-   -- so we need to do the `focus1` here.)
-   (λ d, lock_tactic_state $ focus1 $ do
-     apply_declaration ff opt d,
-     ng ← num_goals,
-     s ← read,
-     m ← tactic_statement g, 
-     return
-     { application .
-       state := s,
-       decl := d.d,
-       script := m,
-       num_goals := ng,
-       hyps_used := hyps.countp(λ h, h.occurs g) }))
+   -- recording the tactic script as a string,
+   -- the number of remaining goals,
+   -- and number of local hypotheses used.
+   let results := defs.mfilter_map (apply_declaration_script g hyps opt),
+   -- Now call `symmetry` and try again.
+   -- (Because we are using `mllist`, this is essentially free if we've already found a lemma.)
+   symm_state ← retrieve $ try_core $ symmetry >> read,
+   let results_symm := match symm_state with
+   | (some s) :=
+     defs.mfilter_map (λ d, retrieve $ set_state s >> apply_declaration_script g hyps opt d)
+   | none := mllist.nil
+   end,
+  return (results.append results_symm))
 
 /--
 The core `suggest` tactic.
@@ -227,9 +254,11 @@ It attempts to apply a declaration from the library,
 then solve new goals using `solve_by_elim`.
 
 It returns a list of `application`s consisting of fields:
-* `state`, a tactic state resulting from the successful application of a declaration from the library,
+* `state`, a tactic state resulting from the successful application of a declaration from
+  the library,
 * `script`, a string of the form `refine ...` or `exact ...` which will reproduce that tactic state,
-* `decl`, an `option declaration` indicating the declaration that was applied (or none, if `solve_by_elim` succeeded),
+* `decl`, an `option declaration` indicating the declaration that was applied
+  (or none, if `solve_by_elim` succeeded),
 * `num_goals`, the number of remaining goals, and
 * `hyps_used`, the number of local hypotheses used in the solution.
 -/
@@ -242,18 +271,21 @@ See `suggest_core`.
 Returns a list of at most `limit` `application`s,
 sorted by number of goals, and then (reverse) number of hypotheses used.
 -/
-meta def suggest (limit : option ℕ := none) (opt : by_elim_opt := { }) : tactic (list application) :=
+meta def suggest (limit : option ℕ := none) (opt : by_elim_opt := { }) : 
+  tactic (list application) :=
 do let results := suggest_core opt,
    -- Get the first n elements of the successful lemmas
    L ← if h : limit.is_some then results.take (option.get h) else results.force,
    -- Sort by number of remaining goals, then by number of hypotheses used.
-   return $ L.qsort(λ d₁ d₂, d₁.num_goals < d₂.num_goals ∨ (d₁.num_goals = d₂.num_goals ∧ d₁.hyps_used ≥ d₂.hyps_used))
+   return $ L.qsort (λ d₁ d₂, d₁.num_goals < d₂.num_goals ∨
+    (d₁.num_goals = d₂.num_goals ∧ d₁.hyps_used ≥ d₂.hyps_used))
 
 /--
 Returns a list of at most `limit` strings, of the form `exact ...` or `refine ...`, which make
 progress on the current goal using a declaration from the library.
 -/
-meta def suggest_scripts (limit : option ℕ := none) (opt : by_elim_opt := { }) : tactic (list string) :=
+meta def suggest_scripts (limit : option ℕ := none) (opt : by_elim_opt := { }) :
+  tactic (list string) :=
 do L ← suggest limit opt,
    return $ L.map application.script
 
@@ -301,6 +333,44 @@ do asms ← mk_assumption_set ff hs attr_names,
     else
       L.mmap trace >> skip
 
+/--
+`suggest` lists possible usages of the `refine` tactic and leaves the tactic state unchanged.
+It is intended as a complement of the search function in your editor, the `#find` tactic, and
+`library_search`.
+
+`suggest` takes an optional natural number `num` as input and returns the first `num` (or less, if
+all possibilities are exhausted) possibilities ordered by length of lemma names.
+The default for `num` is `50`.
+
+For performance reasons `suggest` uses monadic lazy lists (`mllist`). This means that `suggest`
+might miss some results if `num` is not large enough. However, because `suggest` uses monadic
+lazy lists, smaller values of `num` run faster than larger values.
+
+An example of `suggest` in action,
+
+```lean
+example (n : nat) : n < n + 1 :=
+begin suggest, sorry end
+```
+
+prints the list,
+
+```lean
+Try this: exact nat.lt.base n
+Try this: exact nat.lt_succ_self n
+Try this: refine not_le.mp _
+Try this: refine gt_iff_lt.mp _
+Try this: refine nat.lt.step _
+Try this: refine lt_of_not_ge _
+...
+```
+-/
+add_tactic_doc
+{ name        := "suggest",
+  category    := doc_category.tactic,
+  decl_names  := [`tactic.interactive.suggest],
+  tags        := ["search", "Try this"] }
+
 declare_trace silence_library_search -- Turn off `exact ...` trace message for `library_search
 
 /--
@@ -322,8 +392,45 @@ do asms ← mk_assumption_set ff hs attr_names,
    else
      trace
 
+/--
+`library_search` is a tactic to identify existing lemmas in the library. It tries to close the
+current goal by applying a lemma from the library, then discharging any new goals using
+`solve_by_elim`.
+
+Typical usage is:
+```lean
+example (n m k : ℕ) : n * (m - k) = n * m - n * k :=
+by library_search -- Try this: exact nat.mul_sub_left_distrib n m k
+```
+
+`library_search` prints a trace message showing the proof it found, shown above as a comment.
+Typically you will then copy and paste this proof, replacing the call to `library_search`.
+-/
+add_tactic_doc
+{ name        := "library_search",
+  category    := doc_category.tactic,
+  decl_names  := [`tactic.interactive.library_search],
+  tags        := ["search", "Try this"] }
+
 end interactive
 
+/-- Invoking the hole command `library_search` ("Use `library_search` to complete the goal") calls
+the tactic `library_search` to produce a proof term with the type of the hole.
+
+Running it on
+
+```lean
+example : 0 < 1 :=
+{!!}
+```
+
+produces
+
+```lean
+example : 0 < 1 :=
+nat.one_pos
+```
+-/
 @[hole_command] meta def library_search_hole_cmd : hole_command :=
 { name := "library_search",
   descr := "Use `library_search` to complete the goal.",
@@ -331,5 +438,11 @@ end interactive
     script ← library_search,
     -- Is there a better API for dropping the 'exact ' prefix on this string?
     return [((script.mk_iterator.remove 6).to_string, "by library_search")] }
+
+add_tactic_doc
+{ name        := "library_search",
+  category    := doc_category.hole_cmd,
+  decl_names  := [`tactic.library_search_hole_cmd],
+  tags        := ["search", "Try this"] }
 
 end tactic
